Rewrite Cert.v completely, still much work left

assembly/Cert.v
@@ -2,252 +2,202 @@ From Assembly Require Import Mono.
 
 Unset Suggest Proof Using.
 
-(* Does it create more problems than it solves? *)
-(* Set Implicit Arguments. *)
 
 
-(** ** Certified programs *)
+Definition Cert (spec: M bool) :=
+  exists (f: State -> nat), spec ⊑ let* s := get in
+                           nSteps (f s).
 
-Inductive Reach (stop: State) : forall (cont: bool) (start: State), Prop :=
-| Stop s : stop ⊑ s -> Reach stop true s
-| Exit s' s : oneStep s = Some (s', false) -> stop ⊑ s' -> Reach stop false s
-| More c s' s : oneStep s = Some (s', true) -> Reach stop c s' -> Reach stop c s.
+(** In some cases we know exactly how many steps are needed. *)
+Definition nCert n (spec: M bool) := spec ⊑ nSteps n.
 
-Derive Signature for Reach.
-
-Arguments Stop {_} {_}.
-Arguments Exit {_} {_} {_}.
-Arguments More {_} {_} {_} {_}.
-
-Lemma generalize_stop {s1 s2 s3 c} (Hs: s3 ⊑ s2) (Hr: Reach s2 c s1) : Reach s3 c s1.
+Proposition nCert_is_Cert n (spec: M bool) : nCert n spec -> Cert spec.
 Proof.
-  induction Hr as [s1 H | s1' s1 Ho H | c s1' s1 Ho Hr IH];
-    [apply Stop | apply (Exit Ho) | exact (More Ho IH)];
-    transitivity s2; assumption.
+  unfold nCert, Cert.
+  intros H.
+  exists (fun _ => n).
+  rewrite get_ret.
+  exact H.
 Qed.
 
-(* TODO: Why is this needed? *)
-Instance osb_relation : Rel (option (State * bool)) :=
-  option_relation (prod_relation _ eq_relation).
+Definition swallow1 (op: Z) : M unit :=
+  let* pc := get' PC in
+  let* x := load pc in
+  assert* x = toBits 8 op in
+  put' PC (offset 1 pc).
 
-Notation oneStep := (@oneStep Mono.MP1 estParams2).
+Open Scope vector.
 
-Lemma generalize_start {s1 s2 s3 c} (Hr: Reach s3 c s2) (Hs: s2 ⊑s1) : Reach s3 c s1.
-Proof. (* TODO: clean up *)
-  revert s1 Hs.
-  induction Hr as [s2 H | s2' s2 Ho H | c s2' s2 Ho Hr IH]; intros s1 Hs.
-  - apply Stop; transitivity s2; assumption.
-  - assert (oneStep s2 ⊑ oneStep s1) as H_one.
-    + unfold rel, option_relation.
-      exact (oneStep_propr Hs).
-    + clear Hs.
-      rewrite Ho in H_one. clear Ho.
-      destruct (oneStep s1) as [[s1' b]|] eqn:H1.
-      * cbn in H_one.
-        destruct H_one as [Ho1 Ho2].
-        unfold rel, eq_relation in Ho2.
-        subst b.
-        apply (Exit H1).
-        transitivity s2'; assumption.
-      * contradict H_one.
+Equations swallow {n} (ops: vector Z n) : M unit :=
+  swallow [] := ret tt;
+  swallow (op :: rest) :=
+    swallow1 op;;
+    swallow rest.
 
-  - assert (oneStep s2 ⊑ oneStep s1) as H_one.
-    + unfold rel, option_relation.
-      exact (oneStep_propr Hs).
-    + clear Hs.
-      rewrite Ho in H_one. clear Ho.
-      destruct (oneStep s1) as [[s1' b]|] eqn:H1.
-      * cbn in H_one.
-        destruct H_one as [Ho1 Ho2].
-        unfold rel, eq_relation in Ho2.
-        subst b.
-        specialize (IH s1' Ho1).
-        apply (More H1 IH).
-      * contradict H_one.
-Qed.
-
-Lemma reach_comp {s1 s2 s3 t} (H23: Reach s3 t s2) (H12: Reach s2 true s1) : Reach s3 t s1.
+Lemma swallow_action {m n} (o1: vector Z m) (o2: vector Z n) :
+  swallow (o1 ++ o2) = swallow o1;; swallow o2.
 Proof.
-  depind H12.
-  - exact (generalize_start H23 H).
-  - exact (More H (IHReach _ _ H23)).
+  induction m.
+  - dependent elimination o1.
+    simp swallow.
+    smon_rewrite.
+    reflexivity.
+  - dependent elimination o1 as [ @Vector.cons x m o1 ].
+    simpl (swallow _).
+    simp swallow.
+    rewrite (IHm o1).
+    rewrite bind_assoc.
+    reflexivity.
+Qed.
+
+(* TODO: Move *)
+Lemma assert_bind {P} {DP: Decidable P} {X} {mx: M X} {Y} {f: X -> M Y} :
+  (assert* P in mx) >>= f = assert* P in (mx >>= f).
+Proof.
+  destruct (decide P); [ | rewrite err_bind ]; reflexivity.
+Qed.
+
+(* TODO: Move *)
+Lemma assert_bind' {P} {DP: Decidable P} {X} {f: P -> M X} {Y} {g: X -> M Y} :
+  (assert* P as H in f H) >>= g = assert* P as H in (f H >>= g).
+Proof.
+  destruct (decide P); [ | rewrite err_bind ]; reflexivity.
+Qed.
+
+(* TODO: Move *)
+Opaque put'.
+
+Lemma swallow_lemma {n} {ops: vector Z n} {X} {u: M X} {f: Bytes n -> M X} :
+  u ⊑ f (Vector.map toB8 ops) -> swallow ops;; u ⊑ next n >>= f.
+Proof.
+  intros H.
+  repeat setoid_rewrite bind_assoc.
+  revert ops u f H.
+  induction n; intros ops u f H; simp next.
+  - dependent elimination ops. simp swallow.
+    setoid_rewrite ret_bind. exact H.
+  - dependent elimination ops as [Vector.cons (n:=n) x r].
+    simp swallow.
+    unfold swallow1.
+    repeat setoid_rewrite bind_assoc.
+    setoid_rewrite assert_bind.
+    repeat crush.
+    + srel_destruct Hst. assumption.
+    + setoid_rewrite ret_bind.
+      apply IHn. subst y0. exact H.
 Qed.
 
 
-(** ** Cert *)
+(** ** ?? *)
 
-Notation M := (@M _ estParams2).
-
-Class Cert (spec: M bool) :=
-  evidence s:
-    match spec s with
-    | Some (s', b) => Reach s' b s
-    | None => True
-    end.
+(* TODO: Place inside section or module. *)
+Import OpCodes.
 
 Local Notation not_terminated := (ret true) (only parsing).
 Local Notation terminated := (ret false) (only parsing).
 
-(** The empty program has no effect. *)
-Instance cert_id : Cert (not_terminated).
+(* TODO: Move? *)
+Opaque next.
+
+Lemma next_helper (op: Z) (Hop: 0 <= op < 256) :
+  (Vector.map toB8 [op] : Bytes 1) = Z.to_N op :> N.
+Proof. (* TODO: automate? *)
+  simpl Vector.map.
+  remember (toB8 op) as u eqn:Hu.
+  dependent elimination u as [[b0; b1; b2; b3; b4; b5; b6; b7]].
+  simp bytesToBits. simpl. rewrite Hu.
+  unfold bitsToN. f_equal.
+  apply fromBits_toBits. cbn. lia.
+Qed.
+
+Lemma match_helper (op: Z) (Hop: 0 <= op < 256) :
+  Z.of_N (bitsToN (bytesToBits (cells_to_bytes (Vector.map toB8 [op])))) = op.
 Proof.
-  intros s.
-  simpl.
-  apply Stop.
-  unfold PropR.
+  unfold cells_to_bytes, id.
+  rewrite next_helper;
+    [ rewrite Z2N.id | ];
+    lia.
+Qed.
+
+Ltac cert_start :=
+  unfold nCert;
+  simp nSteps;
+  unfold chain, oneStep;
+  setoid_rewrite bind_assoc;
+  try setoid_rewrite bind_assoc;
+  apply swallow_lemma;
+  setoid_rewrite next_helper; [ | lia ];
+  try (unfold cells_to_bytes, id;
+       rewrite next_helper; try lia);
+  simpl;
+  repeat rewrite ret_bind;
+  repeat crush.
+
+Lemma cert_exit : nCert 1 (swallow [EXIT];;
+                           terminated).
+Proof. cert_start. Qed.
+
+Lemma cert_nop : nCert 1 (swallow [NOP];;
+                          not_terminated).
+Proof. cert_start. Qed.
+
+Lemma bind_ret_helper {X Y Z} {mx: M X} {y: Y} {f: Y -> M Z} :
+  mx;; ret y >>= f = mx;; f y.
+Proof.
+  rewrite bind_assoc, ret_bind. reflexivity.
+Qed.
+
+Lemma cert_jump : nCert 1 (swallow [JUMP];;
+                           let* a := pop64 in
+                           put' PC a;;
+                           not_terminated).
+Proof.
+  unfold nCert;
+  simp nSteps;
+  unfold chain, oneStep.
+  setoid_rewrite bind_assoc at 3.
+  apply swallow_lemma.
+  rewrite match_helper; [ | lia ].
+  rewrite bind_ret_helper.
+  rewrite <- bind_assoc.
+  apply (bind_propr _ _); [ | repeat crush ].
+  simp oneStep'.
+  apply (bind_propr _ _); repeat crush.
+  rewrite ofN_bitsToN, toBits_fromBits.
   reflexivity.
 Qed.
 
-Instance cert_comp (u: M bool) {Cu: Cert u} (v: M bool) {Cv: Cert v} :
-  Cert (let* t := u in
-        if t then v else ret false).
+Lemma cert_id : nCert 0 (not_terminated).
 Proof.
-  intros s. specialize (Cu s). simpl.
-  destruct (u s) as [[s' t]|] eqn:Hu; [|exact I].
-  destruct t eqn:Ht.
-  - specialize (Cv s').
-    destruct (v s') as [[s'' t']|] eqn:Hvs; [|exact I].
-    exact (reach_comp Cv Cu).
+  unfold nCert.
+  simp nSteps.
+  repeat crush.
+Qed.
+
+Instance chain_propr : PropR chain.
+Proof.
+  intros u u' Hu v v' Hv.
+  unfold chain.
+  apply (bind_propr _ _).
+  - exact Hu.
+  - intros x x' Hx.
+    cbv in Hx.
+    subst x.
+    destruct x'.
+    + exact Hv.
+    + repeat crush.
+Qed.
+
+Lemma ncert_comp m n (u: M bool) {Cu: nCert m u} (v: M bool) {Cv: nCert n v} :
+  nCert (m + n) (chain u v).
+Proof.
+  unfold nCert in *.
+  rewrite nSteps_action.
+  apply chain_propr.
   - exact Cu.
+  - exact Cv.
 Qed.
 
-
-(** ** Basic certs *)
-
-Instance cert1 {u: M unit} (b: bool)
-         (H: forall s, match u s with
-                  | Some (s', _) => Reach s' b s
-                  | None => True
-                  end) : Cert (u;; ret b).
-Proof.
-  intros s.
-  specialize (H s).
-  simpl.
-  destruct (u s) as [[s' _]|]; exact H.
-Qed.
-
-Equations swallow (ops: list Z) : M unit :=
-  swallow [] := ret tt;
-  swallow (op :: rest) :=
-    let* pc := get' PC in
-    let* x := load pc in
-    assert* x = op :> Z in
-    put' PC (offset 1 pc);;
-    swallow rest.
-
-(* TODO: simplify? *)
-Ltac comp :=
-  repeat (
-      simpl
-    || simp to_list fromLittleEndian toBits bitListToNat).
-
-Ltac cert_start :=
-  apply cert1; intros s;
-  simp swallow; simpl;
-  (destruct load as [[s' x]|] eqn:H1; [|exact I]);
-  (destruct decide; [subst x|exact I]).
-
-Section offset_opaque_section.
-
-  Opaque offset.
-
-  Import OpCodes.
-  Global Instance cert_exit : Cert (swallow [EXIT];;
-                                    terminated).
-  Proof.
-    cert_start.
-    set (stop := update _ _ _).
-    refine (Exit _ ltac:(reflexivity)).
-    unfold oneStep. simpl.
-    rewrite H1. comp.
-    reflexivity.
-  Qed.
-
-  Instance cert_nop: Cert (swallow [NOP];;
-                           not_terminated).
-  Proof.
-    cert_start.
-    set (stop := update _ _ _).
-    refine (More _ (Stop ltac:(reflexivity))).
-    unfold oneStep. simpl.
-    rewrite H1. comp.
-    reflexivity.
-  Qed.
-
-
-(** Assembler jump_zero *)
-
-Equations availableBefore (a: Addr) (n: nat) : M unit :=
-  availableBefore _ 0 := ret tt;
-  availableBefore a (S n) :=
-    assert* (available (offset (S n) a)) in
-    availableBefore a n.
-
-Definition requireStack (n: nat) : M unit :=
-  let* sp := get' SP in
-  availableBefore sp (8 * n).
-
-Definition isZero := [PUSH1; toB8 1; LT].
-
-Definition boolRep (P: Prop) {DP: Decidable P} : Z :=
-  if decide P then (-1)%Z else 0%Z.
-
-Instance cert_isZero : Cert (swallow isZero;;
-                             requireStack 1;;
-                             let* n := popN in
-                             push64 (boolRep (n = 0));;
-                             not_terminated).
-Proof.
-  setoid_rewrite <- bind_assoc at 3.
-  setoid_rewrite <- bind_assoc at 2.
-  setoid_rewrite <- bind_assoc at 1.
-
-  apply cert1. intros s. unfold isZero, requireStack.
-  simpl mult. rewrite swallow_equation_2.
-  (* simp swallow. *)
-  (* Does not work here: simp availableBefore.
-     Neither does: setoid_rewrite availableBefore_equation_2. *)
-
-  simpl.
-  (destruct load as [[s' x]|] eqn:H1; [|exact I]).
-
-
-
-
-  setoid_rewrite bind_assoc.
-
-simpl.
-  (destruct decide; [subst x|exact I]).
-
-  cert_start.
-
-
-
-Definition pushNum (z: Z) :=
-  (* Non-optimized *)
-  PUSH8 :: toLittleEndian 8 z.
-
-Definition pop n :=
-  let pop1 := [JUMP_ZERO; toB8 0] in
-  match n with
-  | 0 => []
-  | 1 => pop1
-  | 2 => pop1 ++ pop1
-  | n => [GET_SP] ++ pushNum (n * 8) ++ [ADD; SET_SP]
-  end.
-
-Definition genericConditional interjection :=
-  [
-    GET_SP; PUSH1; toB8 8; ADD; LOAD8 (* a::x::r -> x::a::x::r *)
-  ] ++ interjection ++ [
-    JUMP_ZERO; toB8 6;
-    (* If not zero: *)
-    GET_SP; PUSH1; toB8 8; ADD; STORE8 (* a::x::r -> a::r *)
-  ] ++ pop 2. (* If zero *)
-
-
-Definition jump_zero_ops :=
-  [
-
-  ]
-End offset_opaque_section.
+(** To be continued.
+It seems possible that we will need an extra axiom at some,
+ensuring that [⊑] is transitive on [M bool], but we'll see. *)
